protocols/Verification/NetAuthSecure2.v
@@ -5,9 +5,7 @@
  * 
  *)
 From Coq Require Import
-     Eqdep
-     List
-     Lia.
+     List.
 
 From SPICY Require Import
      MyPrelude
@@ -31,7 +29,7 @@ From SPICY Require Import
 .
 
 From protocols Require Import
-     PGP.
+     NetAuth.
 
 From SPICY Require IdealWorld RealWorld.
 
@@ -39,31 +37,99 @@ Import IdealWorld.IdealNotations
        RealWorld.RealWorldNotations
        SimulationAutomation.
 
+From Frap Require Import Sets.
+
+Module Foo <: Sets.EMPTY.
+End Foo.
+Module Import SN := Sets.SetNotations(Foo).
+
 Set Implicit Arguments.
 
 Open Scope protocol_scope.
 
-Module PGPProtocolSecure <: AutomatedSafeProtocolSS.
+Module NetAuthProtocolSecure <: AutomatedSafeProtocolSS'.
 
-  Import PGPProtocol.
+  Import NetAuthProtocol.
 
+  (* Some things may need to change here.  t__hon is where we place the 
+   * type that the protocol computes.  It is set to Nat now, because we
+   * return a natual number.
+   *)
   Definition t__hon := Nat.
   Definition t__adv := Unit.
-  Definition b := tt.
+  Definition b    := tt.
+
+  (* These two variables hook up the starting points for both specification and
+   * implementation universes.  If you followed the template above, this shouldn't
+   * need to be changed.
+   *)
   Definition iu0  := ideal_univ_start.
   Definition ru0  := real_univ_start.
 
   Import Gen Tacs.
 
+  (* These are here to help the proof automation.  Don't change. *)
   #[export] Hint Unfold t__hon t__adv b ru0 iu0 ideal_univ_start real_univ_start : core.
+  #[export] Hint Unfold
+       mkiU mkiUsr mkrU mkrUsr
+       mkKeys
+    : core.
+
+  Lemma finitelyRuns : exists n, runningTimeMeasure ru0 n.
+  Proof.
+    autounfold; simpl.
+    eexists.
+    econstructor; simpl; find_runtime.
+
+    Unshelve.
+    all: exact 0.
+  Qed.
+
+  Require Import Coq.Program.Equality.
+
+  Lemma typechecks : syntactically_safe_U ru0.
+  Proof.
+    unfold syntactically_safe_U; intros.
+    autounfold
+    ; subst
+    ; simpl in *.
+
+    unfold compute_ids; simpl.
+
+    focus_user; simpl
+    ; try solve [ do 2 eexists; split
+                  ; [ unshelve (repeat typechecks1)
+                      ; match goal with
+                        | [ |- bool ] => exact true
+                        | [ |- list safe_typ ] => exact []
+                        end
+                    | repeat verify_context_soundness ] ].
+
+
+    Unshelve.
+    all : exact TyDontCare.
+  Qed.
+    
+  Lemma summarizable : exists summaries, summarize_univ ru0 summaries.
+  Proof.
+    autounfold; unfold summarize_univ; simpl; intros.
+    unshelve (
+        eexists; intros; focus_user; simpl
+        ; (exists useless_summary; split; [ build_summary |]; eauto using useless_summary_summarizes)
+      ) ; exact $0.
+  Qed.
+    
+  Lemma lameness : @lameAdv t__adv b (RealWorld.adversary ru0).
+  Proof.
+    unfold lameAdv; autounfold; simpl; eauto.
+  Qed.
 
   Set Ltac Profiling.
 
   Lemma safe_invariant :
     invariantFor
       {| Initial := {(ru0, iu0, true)}; Step := @stepSS t__hon t__adv  |}
-      (@safety_inv t__hon t__adv).
-      (* (fun st => safety st /\ alignment st /\ returns_align st). *)
+      (@noresends_inv t__hon t__adv).
   Proof.
     unfold invariantFor
     ; unfold Initial, Step
@@ -75,18 +141,17 @@ Module PGPProtocolSecure <: AutomatedSafeProtocolSS.
 
     autounfold in H0
     ; unfold fold_left, fst, snd in *.
-    unfold real_users, ideal_users, mkrUsr, userProto, userKeys, userId, mkiUsr in *; rwuf.
-
+    
     time (
         repeat transition_system_step
       ).
 
     Unshelve.
-    all: eauto.
+    all: exact 0  || auto.
   Qed.
 
   Show Ltac Profile.
-      
+
   Lemma U_good : @universe_starts_sane _ Unit b ru0.
   Proof.
     autounfold;
@@ -149,4 +214,4 @@ Module PGPProtocolSecure <: AutomatedSafeProtocolSS.
           eauto.
   Qed.
 
-End PGPProtocolSecure.
+End NetAuthProtocolSecure.
